@prefix rdf: <http://www.w3.org/1999/02/22-rdf-syntax-ns#> .
@prefix rdfs: <http://www.w3.org/2000/01/rdf-schema#> .
@prefix owl: <http://www.w3.org/2002/07/owl#> .
@prefix n: <http://www.w3.org/2006/vcard/ns#>.
@prefix ldp: <http://www.w3.org/ns/ldp#> .
@prefix schema: <http://schema.org/> .
@prefix dcterms: <http://purl.org/dc/terms/> .
@prefix time: <http://www.w3.org/2006/time#> .
@prefix foaf: <http://xmlns.com/foaf/0.1/> .
@prefix xsd: <http://www.w3.org/2001/XMLSchema#> .
@prefix mud: <https://raw.githubusercontent.com/Multi-User-Domain/vocab/main/mud.ttl#> .
@prefix mudlogic: <https://raw.githubusercontent.com/Multi-User-Domain/vocab/main/mudlogic.ttl#> .
@prefix mudchar: <https://raw.githubusercontent.com/Multi-User-Domain/vocab/main/mudchar.ttl#> .
@prefix mudcard: <https://raw.githubusercontent.com/Multi-User-Domain/vocab/main/mudcard.ttl#> .
@prefix mudworld: <https://raw.githubusercontent.com/Multi-User-Domain/vocab/main/mudworld.ttl#> .

@prefix simpolis: <https://raw.githubusercontent.com/Multi-User-Domain/vocab/main/games/simpolis.ttl#> .

simpolis:ProblemGenerationInstruction a rdfs:Class ;
    rdfs:label "ProblemGenerationInstruction"@en ;
    rdfs:comment "Includes terms describing how to find new problems for an AI"@en .

simpolis:generateProblemEndpoint a rdf:Property ;
    rdfs:label "generateProblemEndpoint"@en ;
    rdfs:comment "Indicates the URL where problems can be generated"@en ;
    rdfs:domain simpolis:ProblemGenerationInstruction ;
    rdfs:range schema:URL .

#
#   Needs: a system for needs which are actively maintained, like hunger, as opposed to requirements like oxygen
#

simpolis:Need a rdfs:Class ;
    rdfs:label "Need"@en ;
    rdfs:comment "A value which will deteriorate over time and needs to be maintained by a character"@en .

simpolis:orderNeed a rdf:Property ;
    rdfs:label "orderNeed"@en ;
    rdfs:comment "Lower order needs will be addressed first (e.g. hunger is at zero). See the Wiki for further explanation"@en ;
    rdfs:range xsd:Integer .

# need functions from the perspective of the subject using them

simpolis:hasMetNeeds a rdf:Property ;
    rdfs:label "hasMetNeeds"@en ;
    rdfs:comment "the subject has a container of Needs which are being maintained effectively"@en ;
    rdfs:range ldp:Container .

# TODO: need deterioration consequences

simpolis:hasEmergencyNeeds a rdf:Property ;
    rdfs:label "hasEmergencyNeeds"@en ;
    rdfs:comment "the subject has a container of Needs which are not being met to the extent that they are in danger"@en ;
    rdfs:range ldp:Container .

# core game Needs

simpolis:Hunger a simpolis:Need ;
    simpolis:orderNeed 0 .
