@prefix rdf: <http://www.w3.org/1999/02/22-rdf-syntax-ns#> .
@prefix rdfs: <http://www.w3.org/2000/01/rdf-schema#> .
@prefix owl: <http://www.w3.org/2002/07/owl#> .
@prefix ldp: <http://www.w3.org/ns/ldp#> .
@prefix schema: <http://schema.org/> .
@prefix dcterms: <http://purl.org/dc/terms/> .
@prefix time: <http://www.w3.org/2006/time#> .
@prefix foaf: <http://xmlns.com/foaf/0.1/> .
@prefix xsd: <http://www.w3.org/2001/XMLSchema#> .
@prefix mud: <https://raw.githubusercontent.com/Multi-User-Domain/vocab/main/mud.ttl#> .
@prefix mudlogic: <https://raw.githubusercontent.com/Multi-User-Domain/vocab/main/mudlogic.ttl#> .
@prefix mudchar: <https://raw.githubusercontent.com/Multi-User-Domain/vocab/main/mudchar.ttl#> .
@prefix mudcard: <https://raw.githubusercontent.com/Multi-User-Domain/vocab/main/mudcard.ttl#> .
@prefix mudworld: <https://raw.githubusercontent.com/Multi-User-Domain/vocab/main/mudworld.ttl#> .

@prefix twt2023: <https://raw.githubusercontent.com/Multi-User-Domain/vocab/main/games/twt2023.ttl#> .

twt2023:RecordedHistory a rdfs:Class ;
    rdfs:label "Recorded History"@en ;
    rdfs:comment "A class for recording history in the world"@en .

twt2023:hasRecordedHistory a rdf:Property ;
    rdfs:label "hasRecordedHistory"@en ;
    rdfs:comment "Intended for world - the log of what happens in the world"@en ;
    rdfs:range ldp:Container .

twt2023:lordOfRegion a rdf:Property ;
    rdfs:label "Lord of Region"@en ;
    rdfs:comment "Indicates that the subject character is the lord of the object region"@en ;
    rdfs:domain mudchar:Character ;
    rdfs:range mudworld:Region .

twt2023:huntsInRegion a rdf:Property ;
    rdfs:label "feedsInRegion"@en ;
    rdfs:comment "Indicates that the subject uses a list of regions (regularly) to hunt"@en ;
    rdfs:range ldp:Container .

twt2023:generatesCardFrom a rdf:Property ;
    rdfs:label "generatesCardFrom"@en ;
    rdfs:comment "Specifically for card generating Actions and Effects, indicates the possible cards to generate from"@en ;
    rdfs:domain mudlogic:Action ;
    rdfs:range ldp:Container .

# TODO: not implemented Godot side
#twt2023:generatesCardTo a rdf:Property ;
#    rdfs:label "generatesCardTo"@en ;
#    rdfs:comment "Where the card is generated to. Expected to be a player, i.e. into my deck or that of my opponent"@en ;
#    rdfs:domain mudlogic:Action .

# TODO: replace below with mudlogic property
twt2023:maximumUses a rdf:Property ;
    rdfs:label "maximumUses"@en ;
    rdfs:comment "Indicates that an action can only be used a certain number of times"@en ;
    rdfs:range xsd:Integer .

twt2023:hasAvailableEvents a rdf:Property ;
    rdfs:label "hasAvailableEvents"@en ;
    rdfs:comment "A list of events which can be triggered by the card"@en ;
    rdfs:range ldp:Container .

twt2023:generateCardProbability a rdf:Property ;
    rdfs:label "generateCardProbability"@en ;
    rdfs:comment "on the Action, indicates how likely it is that a card will be selected at all"@en ;
    rdfs:range xsd:Decimal .

twt2023:onGeneratedMessage a rdf:Property ;
    rdfs:label "onGeneratedMessage"@en ;
    rdfs:comment "an optional message when the card is generated, announcing its' entrance"@en ;
    rdfs:range xsd:String .

twt2023:DuplicateSelf a mudlogic:Effect .
