@prefix rdf: <http://www.w3.org/1999/02/22-rdf-syntax-ns#> .
@prefix rdfs: <http://www.w3.org/2000/01/rdf-schema#> .
@prefix owl: <http://www.w3.org/2002/07/owl#> .
@prefix dcterms: <http://purl.org/dc/terms/> .
@prefix xsd: <http://www.w3.org/2001/XMLSchema#> .
@prefix mudlogic: <https://raw.githubusercontent.com/Multi-User-Domain/vocab/main/mudlogic.ttl#> .

@prefix mudcombat: <https://raw.githubusercontent.com/Multi-User-Domain/vocab/main/mudcombat.ttl#> .

mudcombat: rdf:type owl:Ontology ;
    # Description
    dcterms:title "Multi-User Domain Combat ontology" ;
    dcterms:description """
    Provides definitions for a commonly used combat system mechanics
    """ ;
    # Ownership
    dcterms:license <http://creativecommons.org/licenses/by/4.0/> ;
    dcterms:creator <https://calum.inrupt.net/profile/card#me> .

mudcombat:PointResource a rdfs:Class ;
    rdfs:label "PointResource"@en ;
    rdfs:comment "A point resource like Health or Mana. Expected to be an integer or a decimal"@en .
    # use n:fn for point resource type name

mudcombat:maximumP a rdf:Property ;
    rdfs:label "maximumP"@en ;
    rdfs:comment "The maximum value of the point resource"@en ;
    rdfs:domain mudcombat:PointResource ;
    rdfs:range xsd:Integer, xsd:Decimal .

mudcombat:currentP a rdf:Property ;
    rdfs:label "currentP"@en ;
    rdfs:comment "The current value of the point resource" ;
    rdfs:domain mudcombat:PointResource ;
    rdfs:range xsd:Integer, xsd:Decimal .

mudcombat:hasPointResourceStats a rdf:Property ;
    rdfs:label "hasPointResourceStats"@en ;
    rdfs:comment "Indicates that the agent has a point resource"@en ;
    rdfs:range mudcombat:PointResource .

# instances for commonly used point resource types

mudcombat:HealthPoints a rdfs:Class ;
    rdfs:subClassOf mudcombat:PointResource ;
    rdfs:label "Health Points"@en ;
    rdfs:comment "Health Points, represents life force"@en .

mudcombat:hasHealthPoints a rdf:Property ;
    rdfs:subPropertyOf mudcombat:PointResource ;
    rdfs:label "hasHealthPoints"@en ;
    rdfs:comment "Health Points. Has its own property because it's commonly used"@en ;
    rdfs:range mudcombat:HealthPoints .

mudcombat:ManaPointsType a rdfs:Class ;
    rdfs:subClassOf mudcombat:hasPointResourceStats ;
    rdfs:label "Mana Points"@en ;
    rdfs:comment "Mana Points, represents magical force"@en .

mudcombat:hasManaPoints a rdf:Property ;
    rdfs:subPropertyOf mudcombat:hasPointResourceStats ;
    rdfs:label "hasManaPoints"@en ;
    rdfs:comment "Mana Points. Has its own property because it's commonly used"@en ;
    rdfs:range mudcombat:ManaPoints .

# Attacks - points consequences modelled using actions/tasks

mudcombat:AttackDetails a rdfs:Class ;
    rdfs:label "AttackDetails"@en ;
    rdfs:comment "Attacks are modelled using actions/tasks, with additional details for their point consequences"@en .

mudcombat:hasAttackDetails a rdf:Property ;
    rdfs:label "hasAttackDetails"@en ;
    rdfs:comment "Property on action/task indicates the straightforward consequences on points systems"@en ;
    rdfs:range mudcombat:AttackDetails .

mudcombat:fixedDamage a rdf:Property ;
    rdfs:label "fixedDamage"@en ;
    rdfs:comment "The attack does fixed damage"@en ;
    rdfs:domain mudcombat:AttackDetails ;
    rdfs:range xsd:Decimal .

mudcombat:minDamage a rdf:Property ;
    rdfs:label "minDamage"@en ;
    rdfs:comment "The attack does variable damage and this is the minimum"@en ;
    rdfs:domain mudcombat:AttackDetails ;
    rdfs:range xsd:Decimal .

mudcombat:maxDamage a rdf:Property ;
    rdfs:label "maxDamage"@en ;
    rdfs:comment "The attack does variable damage and this is the maximum"@en ;
    rdfs:domain mudcombat:AttackDetails ;
    rdfs:range xsd:Decimal .

mudcombat:recurringDamage a rdf:Property ;
    rdfs:label "recurringDamage"@en ;
    rdfs:comment "Indicates the value of fixed damage done on a recurring basis"@en ;
    rdfs:domain mudcombat:AttackDetails ;
    rdfs:range xsd:Decimal .

mudcombat:recurringDamageDuration a rdf:Property ;
    rdfs:label "recurringDamageDuration"@en ;
    rdfs:comment "Indicates the number of seconds the recurring damage goes on for"@en ;
    rdfs:range xsd:Integer .

mudcombat:attackDamagesPoints a rdf:Property ;
    rdfs:label "attackDamagesPoints"@en ;
    rdfs:comment "Indicates that an attack (an action/task from mudlogic) will damage a point resource with the type indicated in the URL"@en ;
    rdfs:range schema:URL .

# Attacks can imbue effects on their target
# NOTE: this can be done via action consequences but is offered in this ontology as a shortcut

mudcombat:imbuesEffects a rdf:Property ;
    rdfs:label "imbuesEffects"@en ;
    rdfs:comment "When the attack is completed it might activate mudlogic:Effects on the target"@en ;
    rdfs:range ldp:Container .

# Attacks deal types of damage

mudcombat:DamageType a rdfs:Class ;
    rdfs:label "Damage Type"@en ;
    rdfs:comment "The type of damage (e.g. physical, poison, fire)"@en .

mudcombat:typeDamage a rdf:Property ;
    rdfs:label "typeDamage"@en ;
    rdfs:comment "Indicates the type of damage done by an attack"@en ;
    rdfs:range mudcombat:DamageType .

# Characters can have resistance to damage types

mudcombat:DamageResistance a rdfs:Class ;
    rdfs:label "Damage Resistance"@en ;
    rdfs:comment "Like DamageType, but protection against"@en .

mudcombat:hasResistances a rdf:Property ;
    rdfs:label "hasResistances"@en ;
    rdfs:comment "Indicates that the subject has a set of Resistances to damage types"@en ;
    rdfs:range ldp:Container .

mudcombat:resistanceValue a rdf:Property ;
    rdfs:label "resistanceValue"@en ;
    rdfs:comment "The value of the resistance in damage percentage -1.0 to 1.0. For weakness set a negative value"@en ;
    rdfs:range xsd:Decimal .

# Some basic types of damage to start with

mudcombat:PhysicalDamage a mudcombat:DamageType .
mudcombat:FireDamage a mudcombat:DamageType .
mudcombat:EarthDamage a mudcombat:DamageType .
mudcombat:WaterDamage a mudcombat:DamageType .
mudcombat:AirDamage a mudcombat:DamageType .
mudcombat:RadiantDamage a mudcombat:DamageType .
mudcombat:NecraticDamage a mudcombat:DamageType .
mudcombat:PoisonDamage a mudcombat:DamageType .
