@prefix rdf: <http://www.w3.org/1999/02/22-rdf-syntax-ns#> .
@prefix rdfs: <http://www.w3.org/2000/01/rdf-schema#> .
@prefix owl: <http://www.w3.org/2002/07/owl#> .
@prefix ldp: <http://www.w3.org/ns/ldp#> .
@prefix schema: <http://schema.org/> .
@prefix dcterms: <http://purl.org/dc/terms/> .
@prefix time: <http://www.w3.org/2006/time#> .
@prefix foaf: <http://xmlns.com/foaf/0.1/> .
@prefix vgo: <http://purl.org/net/videogameontology#> .
@prefix xsd: <http://www.w3.org/2001/XMLSchema#> .
@prefix mud: <https://raw.githubusercontent.com/Multi-User-Domain/vocab/main/mud.ttl#> .
@prefix mudlogic: <https://raw.githubusercontent.com/Multi-User-Domain/vocab/main/mudlogic.ttl#> .
@prefix mudchar: <https://raw.githubusercontent.com/Multi-User-Domain/vocab/main/mudchar.ttl#> .

@prefix mudcard: <https://raw.githubusercontent.com/Multi-User-Domain/vocab/main/mudcard.ttl#> .

mudcard: rdf:type owl:Ontology ;
    # Description
    dcterms:title "Multi-User Domain Card ontology" ;
    dcterms:description """
    Vocabulary containing terms for card games
    """ ;
    # Ownership
    dcterms:license <http://creativecommons.org/licenses/by/4.0/> ;
    dcterms:creator <https://calum.inrupt.net/profile/card#me> .

mudcard:playableCard a mud:Specification .

mudcard:playTarget a rdf:Property ;
    rdfs:label "playTarget"@en ;
    rdfs:comment "Instructs the game how the card should be played (e.g. on a board, on a character, on nothing)"@en .

mudcard:Deck a rdfs:Class ;
    rdfs:label "Deck"@en ;
    rdfs:comment "A deck of cards"@en .

mudcard:cardsAtUrl a rdf:Property ;
    rdfs:label "cardsAtUrl"@en ;
    rdfs:comment "Indicates a URL which when followed defines a list of cards belonging to the deck"@en ;
    rdfs:range schema:URL .

mudcard:hasCards a rdf:Property ;
    rdfs:label "hasCards"@en ;
    rdfs:comment "Possession of a list of cards. Intended for decks to indicate their membership"@en ;
    rdfs:range ldp:Container .

mudcard:hasDeck a rdf:Property ;
    rdfs:label "hasDeck"@en ;
    rdfs:comment "Indicates the subject possesses the object deck"@en ;
    rdfs:range mudcard:Deck .

mudcard:hasAvailableInstantActions a rdf:Property ;
    rdfs:label "hasAvailableInstantActions"@en ;
    rdfs:comment "Indicates the instant actions available to a subject"@en ;
    rdfs:range ldp:Container .

mudcard:hasAvailableIntervalActions a rdf:Property ;
    rdfs:label "hasAvailableIntervalActions"@en ;
    rdfs:comment "Indicates the interval actions (tasks which take time) available to a subject"@en ;
    rdfs:range ldp:Container .
