@prefix rdf: <http://www.w3.org/1999/02/22-rdf-syntax-ns#> .
@prefix rdfs: <http://www.w3.org/2000/01/rdf-schema#> .
@prefix owl: <http://www.w3.org/2002/07/owl#> .
@prefix schema: <http://schema.org/> .
@prefix dcterms: <http://purl.org/dc/terms/> .
@prefix xsd: <http://www.w3.org/2001/XMLSchema#> .
@prefix foaf: <http://xmlns.com/foaf/0.1/> .
@prefix mud: <https://raw.githubusercontent.com/Multi-User-Domain/vocab/main/mud.ttl#> .

@prefix mudcontent: <#> .

mudcontent: rdf:type owl:Ontology ;
    # Description
    dcterms:title "Multi-User Domain Content ontology" ;
    dcterms:description """
    Includes definitions for content in Multi-User Domains
    """ ;
    # Ownership
    dcterms:license <http://creativecommons.org/licenses/by/4.0/> ;
    dcterms:creator <https://matttennison.inrupt.net/profile/card#me> ;
    dcterms:contributor <https://calum.inrupt.net/profile/card#me> .

mudcontent:Content a rdfs:Class ;
  rdfs:label "Content"@en ;
  rdfs:comment "Holds properties for content to render with the object it describes"@en .

mudcontent:Sense a rdfs:Class ;
  rdfs:label "Sense"@en ;
  rdfs:comment "The faculty with which an Actor perceives something"@en.

mudcontent:Sight a mudcontent:Sense ;
  rdfs:label "Sight"@en ;
  rdfs:comment "The visual sense" @en ;
  rdfs:subClassOf mudcontent:Sense .

mudcontent:usesSense a rdf:Property ;
  rdfs:label "usesSense"@en ;
  rdfs:comment "Implies that the subject (Content) uses this Sense"@en ;
  rdfs:range mudcontent:Sense .

mudcontent:hasSense a rdf:Property ;
  rdfs:label "hasSense"@en ;
  rdfs:comment "Connects a Sense to its' perceiver"@en ;
  rdfs:range mudcontent:Sense .

mudcontent:sees a rdf:Property ;
  rdfs:label "Sees"@en ;
  rdfs:comment "The visual sense of the perceiver"@en ;
  rdfs:range mud:Content .

mudcontent:senseStrength a rdf:Property ;
  rdfs:label "senseStrength"@en ;
  rdfs:comment "Used to model whether the perceiver has a heightened or weakened sense of sight, for example. Intended for a gaming context. 0 should be considered normal, and default"@en ;
  rdfs:domain mudcontent:Sense ;
  rdfs:range xsd:integer .

mudcontent:describes a rdf:Property ;
  rdfs:label "Describes"@en ;
  rdfs:comment "The owl:Thing which is being described by the Content"@en ;
  rdfs:domain mudcontent:Content ;
  rdfs:range owl:Thing, schema:URL .

mudcontent:hasText a rdf:Property ;
  rdfs:label "hasText"@en ;
  rdfs:comment "Textual content associated with a Content resource"@en ;
  rdfs:domain mudcontent:Content ;
  rdfs:range xsd:string .

mudcontent:hasImage a rdf:Property ;
  rdfs:subPropertyOf foaf:depiction ;
  rdfs:label "hasImage"@en ;
  rdfs:comment "Image content associated with a Content resource"@en ;
  rdfs:domain mudcontent:Content .

mudcontent:originatesFrom a rdf:Property ;
  rdfs:label "originatesFrom"@en ;
  rdfs:comment "Some content can have an origin source - e.g. a sound might be caused by a character who is speaking. Generally, this is for UI purposes of displaying to the player who did something"@en ;
  rdfs:domain mudcontent:Content ;
  rdfs:range owl:Thing, schema:URL .

mudcontent:sceneDescriptionEndpoint a rdf:Property ;
    rdfs:label "sceneDescriptionEndpoint"@en ;
    rdfs:comment "The URL where a supported scene description endpoint can be found"@en ;
    rdfs:domain mud:Configuration ;
    rdfs:range schema:URL .

mudcontent:simpleObjectDescriptionEndpoint a rdf:Property ;
    rdfs:label "simpleObjectDescriptionEndpoint"@en ;
    rdfs:comment "The URL where a supported simple object description endpoint can be found"@en ;
    rdfs:domain mud:Configuration ;
    rdfs:range schema:URL .
