@prefix rdf: <http://www.w3.org/1999/02/22-rdf-syntax-ns#> .
@prefix rdfs: <http://www.w3.org/2000/01/rdf-schema#> .
@prefix owl: <http://www.w3.org/2002/07/owl#> .
@prefix ldp: <http://www.w3.org/ns/ldp#> .
@prefix schema: <http://schema.org/> .
@prefix dcterms: <http://purl.org/dc/terms/> .
@prefix time: <http://www.w3.org/2006/time#> .
@prefix foaf: <http://xmlns.com/foaf/0.1/> .
@prefix xsd: <http://www.w3.org/2001/XMLSchema#> .
@prefix sh: <http://www.w3.org/ns/shacl#> .
@prefix mud: <https://raw.githubusercontent.com/Multi-User-Domain/vocab/main/mud.ttl#> .

@prefix muddialogue: <#> .

muddialogue: rdf:type owl:Ontology ;
    # Description
    dcterms:title "Multi-User Domain Dialogue ontology" ;
    dcterms:description """
    Vocabulary used in the definitions of decentralised parts of dialogue with characters
    """ ;
    # Ownership
    dcterms:license <http://creativecommons.org/licenses/by/4.0/> ;
    dcterms:creator <https://calum.inrupt.net/profile/card#me> .

# classes and properties for describing the context of a dialogue

muddialogue:Interaction a rdfs:Class ;
    rdfs:label "Interaction"@en ;
    rdfs:label "Échange"@fr ;
    rdfs:comment "Describes the context of a dialogue"@en ;
    rdfs:comment "La contexte d'un échange entre plusieurs acteurs"@fr .

muddialogue:inkFile a rdf:Property ;
    rdfs:label "Ink File"@en ;
    rdfs:comment "Ink is a syntax for writing a script for an interaction"@en ;
    rdfs:range schema:URL .

# NOTE: for deciding whether an interaction can be used in a scene, we can use shapes.
# To model this use the property mudlogic:parameterConstraintsShape

# Bindings: connecting a graph to actors within a game scene

muddialogue:Binding a rdfs:Class ;
    rdfs:label "Binding"@en ;
    rdfs:comment "A resource which is bound to the input or output graph of an ink dialogue"@en .

muddialogue:InkVariableBinding a rdfs:Class ;
    rdfs:subClassOf muddialogue:Binding ;
    rdfs:label "Ink Variable Binding"@en ;
    rdfs:comment "A binding to a variable used in an Ink story"@en .

muddialogue:inkVariableName a rdf:Property ;
    rdfs:label "inkVariableName"@en ;
    rdfs:comment "The value indicates the name of the variable used in a connected Ink story"@en ;
    rdfs:domain muddialogue:InkVariableBinding ;
    rdfs:range xsd:string .

muddialogue:hasBindings a rdf:Property ;
    rdfs:label "hasBindings"@en ;
    rdfs:comment "Contains bindings used to map game logic to the Interaction represented in Linked Data"@en ;
    rdfs:domain muddialogue:Interaction ;
    # TODO: add formal constraint that container should contain only Binding subclasses
    rdfs:range ldp:Container .

muddialogue:bindingMadeToShape a rdf:Property ;
    rdfs:label "bindingMadeToShape"@en ;
    rdfs:comment "A shape which describes the object which the binding should be made to"@en ;
    rdfs:domain muddialogue:Binding ;
    rdfs:range sh:NodeShape .

muddialogue:generateNarrativeContextEndpoint a rdf:Property ;
    rdfs:label "generateNarrativeContextEndpoint"@en ;
    rdfs:comment "An optional link to an endpoint which can be used to generate/complete the graph context needed to run the Interaction"@en ;
    rdfs:domain muddialogue:Interaction ;
    rdfs:range schema:URL .

# classes and properties for describing messages in a dialogue

muddialogue:Message a rdfs:Class ;
    rdfs:label "Dialogue Message"@en ;
    rdfs:comment ""@en .

muddialogue:performer a rdf:Property ;
    rdfs:label "performer"@en ;
    rdfs:comment "The agent communicating a muddialogue:Message"@en ;
    rdfs:domain muddialogue:Message .

muddialogue:content a rdf:Property ;
    rdfs:label "content"@en ;
    rdfs:comment "The content of the muddialogue:Message. What is being said"@en ;
    rdfs:domain muddialogue:Message .

muddialogue:shorthand a rdf:Property ;
    rdfs:label "shorthand description"@en ;
    rdfs:comment "Describes the content in shorter form, e.g. to display the message as a response choice"@en ;
    rdfs:domain muddialogue:Message .

muddialogue:includeContinuePrompt a rdf:Property ;
    rdfs:label "continue prompt"@en ;
    rdfs:comment "If set to true, the client is being advised to provide a continue prompt after the message to break up the conversation"@en ;
    rdfs:range xsd:boolean .

muddialogue:selectFollowup a rdf:Property ;
    rdfs:label "preselected followup"@en ;
    rdfs:comment "If provided, it is signalling to the client that the response for a message can be found my making a GET request to the provided URL. Therefore generally only included if the message is a player response to an NPC"@en ;
    rdfs:range schema:URL .

muddialogue:getResponses a rdf:Property ;
    rdfs:label "get responses URL"@en ;
    rdfs:comment "If provided, it is signalling to the client that the response options for a message can be found my making a GET request to the provided URL. Therefore generally only included if the message is an NPC response to a player"@en ;
    rdfs:range schema:URL .

muddialogue:responses a rdf:Property ;
    rdfs:label "responses list"@en ;
    rdfs:comment "If provided, it is signalling to the client that the response options for a message are defined by the container value"@en ;
    rdfs:range ldp:Container .
