@prefix rdf: <http://www.w3.org/1999/02/22-rdf-syntax-ns#> .
@prefix rdfs: <http://www.w3.org/2000/01/rdf-schema#> .
@prefix owl: <http://www.w3.org/2002/07/owl#> .
@prefix ldp: <http://www.w3.org/ns/ldp#> .
@prefix schema: <http://schema.org/> .
@prefix dcterms: <http://purl.org/dc/terms/> .
@prefix time: <http://www.w3.org/2006/time#> .
@prefix foaf: <http://xmlns.com/foaf/0.1/> .
@prefix xsd: <http://www.w3.org/2001/XMLSchema#> .
@prefix mud: <https://raw.githubusercontent.com/Multi-User-Domain/vocab/main/mud.ttl#> .

@prefix muddialogue: <#> .

muddialogue:Message a rdfs:Class ;
    rdfs:label "Dialogue Message"@en ;
    rdfs:comment ""@en .

muddialogue:performer a rdf:Property ;
    rdfs:label "performer"@en ;
    rdfs:comment "The agent communicating a muddialogue:Message"@en ;
    rdfs:domain muddialogue:Message .

muddialogue:content a rdf:Property ;
    rdfs:label "content"@en ;
    rdfs:comment "The content of the muddialogue:Message. What is being said"@en ;
    rdfs:domain muddialogue:Message .

muddialogue:shorthand a rdf:Property ;
    rdfs:label "shorthand description"@en ;
    rdfs:comment "Describes the content in shorter form, e.g. to display the message as a response choice"@en ;
    rdfs:domain muddialogue:Message .

muddialogue:includeContinuePrompt a rdf:Property ;
    rdfs:label "continue prompt"@en ;
    rdfs:comment "If set to true, the client is being advised to provide a continue prompt after the message to break up the conversation"@en ;
    rdfs:range xsd:boolean .

muddialogue:selectFollowup a rdf:Property ;
    rdfs:label "preselected followup"@en ;
    rdfs:comment "If provided, it is signalling to the client that the response for a message can be found my making a GET request to the provided URL. Therefore generally only included if the message is a player response to an NPC"@en ;
    rdfs:range schema:URL .

muddialogue:getResponses a rdf:Property ;
    rdfs:label "get responses URL"@en ;
    rdfs:comment "If provided, it is signalling to the client that the response options for a message can be found my making a GET request to the provided URL. Therefore generally only included if the message is an NPC response to a player"@en ;
    rdfs:range schema:URL .

muddialogue:responses a rdf:Property ;
    rdfs:label "responses list"@en ;
    rdfs:comment "If provided, it is signalling to the client that the response options for a message are defined by the container value"@en ;
    rdfs:range ldp:Container .
