@prefix rdf: <http://www.w3.org/1999/02/22-rdf-syntax-ns#> .
@prefix rdfs: <http://www.w3.org/2000/01/rdf-schema#> .
@prefix owl: <http://www.w3.org/2002/07/owl#> .
@prefix ldp: <http://www.w3.org/ns/ldp#> .
@prefix schema: <http://schema.org/> .
@prefix dcterms: <http://purl.org/dc/terms/> .
@prefix time: <http://www.w3.org/2006/time#> .
@prefix foaf: <http://xmlns.com/foaf/0.1/> .
@prefix xsd: <http://www.w3.org/2001/XMLSchema#> .
@prefix mud: <https://raw.githubusercontent.com/Multi-User-Domain/vocab/main/mud.ttl#> .

@prefix mudworld: <#> .

mud: rdf:type owl:Ontology ;
    # Description
    dcterms:title "Multi-User Domain World ontology" ;
    dcterms:description """
    An ontology for describing the properties basic to world data in Multi-User Domains
    """ ;
    # Ownership
    dcterms:license <http://creativecommons.org/licenses/by/4.0/> ;
    dcterms:creator <https://calum.inrupt.net/profile/card#me> .

mudworld:Location a rdfs:Class ;
    rdfs:subClassOf mud:Locatable ;
    rdfs:label "Location"@en ;
    rdfs:label "Endroit"@fr ;
    rdfs:comment "A generic setting for a scene"@en .

mudworld:Region a rdfs:Class ;
    rdfs:subClassOf mud:Locatable ;
    rdfs:label "Region"@en ;
    rdfs:label "Région"@fr .

mudworld:Tile a rdfs:Class ;
    rdfs:label "Tile"@en ;
    rdfs:comment "A tile on a tile map"@en .

mudworld:Terrain a rdfs:Class ;
    rdfs:label "Terrain"@en ;
    rdfs:label "Terrain"@fr ;
    rdfs:comment "Represents a type of terrain on a map (e.g. grass, lava)"@en ;
    rdfs:comment "Signifie un genre du terrain sur la carte (e.g. herbe, lave)"@fr .

mudworld:hasRegions a rdf:Property ;
    rdfs:label "hasRegions"@en ;
    rdfs:comment "An ldp:Container defining the sub regions contained within this region. Considered to be a complete set"@en ;
    rdfs:comment "Un ldp:Container définissant les sous-régions contenues dans cette région. Considéré comme un ensemble complet"@fr ;
    rdfs:domain mudworld:Region ;
    rdfs:range ldp:Container .

mudworld:hasVisitable a rdf:Property ;
    rdfs:label "hasVisitable"@en ;
    rdfs:comment "Denotes a link to a visitable location within the Thing"@en ;
    rdfs:comment "Indique un lien vers un lieu visitable au sein de la Thing"@fr .

# providing your world with a map: https://github.com/Multi-User-Domain/vocab/wiki/World-Maps

mudworld:hasTileMap a rdf:Property ;
    rdfs:label "hasTileMap"@en ;
    rdfs:comment "A 2D array describing a grid of tiles (used commonly in 2D games)"@en ;
    rdfs:range ldp:Container .

mudworld:hasTerrain a rdf:Property ;
    rdfs:label "hasTerrain"@en ;
    rdfs:comment "indicates the type of terrain, e.g. on a tile"@en ;
    rdfs:range mudworld:Terrain .

# giving objects location in the world: https://github.com/Multi-User-Domain/vocab/wiki/World-Giving-Things-Location

mudworld:hasSize a rdf:Property ;
    rdfs:label "hasSize"@en ;
    rdfs:comment "the 2D or 3D size of an object, measured in cells"@en .

mudworld:hasMapInhabitants a rdf:Property ;
    rdfs:label "hasMapInhabitants"@en ;
    rdfs:comment "An array of objects which exist within the map space (e.g. characters and buildings). Represented by their coordinates and by their data"@en ;
    rdfs:range ldp:Container .

mudworld:inhabitantData a rdf:Property ;
    rdfs:label "inhabitantData"@en ;
    rdfs:comment "points to an object which describes the inhabitant data (e.g. a character or building)"@en .

# Populations
# use the mud:species property to indicate which species the population represents

mudworld:Population a rdfs:Class ;
    rdfs:label "Population"@en ;
    rdfs:label "Population"@fr ;
    rdfs:comment "A population of a species."@en ;
    rdfs:comment "Une population d'une espèce."@fr .

mudworld:populationNumber a rdf:Property ;
    rdfs:label "Population Number"@en ;
    rdfs:label "Nombre Population"@fr ;
    rdfs:comment "The integer number of a population."@en ;
    rdfs:comment "Le nombre entier de la population."@fr ;
    rdfs:domain mudworld:Population ;
    rdfs:range xsd:integer .

mudworld:hasPopulations a rdf:Property ;
    rdfs:label "hasPopulations"@en ;
    rdfs:label "hasPopulations"@fr ;
    rdfs:comment "Indicates that the subject thing (e.g. Region) has the populations of the object ldp:Container"@en ;
    rdfs:comment "Indique que le sujet (e.g. Région), a des populations stockées dans l'objet ldp:Container"@fr ;
    rdfs:range ldp:Container .
